src/simulation/ModSim.v
@@ -1281,6 +1281,80 @@ End PRIMIVIESIM.
 #[export] Hint Resolve lsim_mon: paco.
 #[export] Hint Resolve cpn9_wcompat: paco.
 
+Section EQUIVI.
+
+  Context `{M: URA.t}.
+
+  Variable state_src: Type.
+  Variable state_tgt: Type.
+
+  Variable ident_src: ID.
+  Variable _ident_tgt: ID.
+  Local Notation ident_tgt := (ident_tgt _ident_tgt).
+
+  Variable wf_src: WF.
+  Variable wf_tgt: WF.
+
+  Let srcE := threadE ident_src state_src.
+  Let tgtE := threadE _ident_tgt state_tgt.
+
+  Local Notation shared := (shared state_src state_tgt ident_src _ident_tgt wf_src wf_tgt).
+
+  Let shared_rel: Type := shared -> Prop.
+  (* Variable I: shared -> URA.car -> Prop. *)
+
+  Lemma __lsim_equivI tid
+        (I1 I2 : shared -> URA.car -> Prop)
+        (EQ : forall shr (m : URA.car) (WF : URA.wf m), I1 shr m <-> I2 shr m)
+    :
+    __lsim I1 tid <11= __lsim I2 tid.
+  Proof.
+    i. ss. inv PR; try (econs; eauto; fail).
+    { eapply lsim_yieldR.
+      - eapply EQ. 2: apply INV. do 2 eapply URA.wf_mon. eauto.
+      - eauto.
+      - i. eapply LSIM. 3: apply TGT. 2: apply VALID0. apply EQ; auto. do 2 eapply URA.wf_mon. eauto.
+    }
+    { eapply lsim_sync.
+      - eapply EQ. 2: apply INV. do 2 eapply URA.wf_mon. eauto.
+      - eauto.
+      - i. eapply LSIM. 3: apply TGT. 2: apply VALID0. apply EQ; auto. do 2 eapply URA.wf_mon. eauto.
+    }
+  Qed.
+
+  Lemma _lsim_equivI tid
+        (I1 I2 : shared -> URA.car -> Prop)
+        (EQ : forall shr (m : URA.car) (WF : URA.wf m), I1 shr m <-> I2 shr m)
+        r
+    :
+    pind9 (__lsim I1 tid r) top9
+    <9=
+      pind9 (__lsim I2 tid r) top9.
+  Proof.
+    i. eapply pind9_mon_gen. eapply PR. 2: auto.
+    i. eapply __lsim_equivI; eauto.
+  Qed.
+
+  Lemma lsim_equivI tid
+        (I1 I2 : shared -> URA.car -> Prop)
+        (EQ : forall shr (m : URA.car) (WF : URA.wf m), I1 shr m <-> I2 shr m)
+    :
+    gupaco9 (fun r => pind9 (__lsim I1 tid r) top9) (cpn9 (fun r => pind9 (__lsim I1 tid r) top9))
+            <10=
+      gupaco9 (fun r => pind9 (__lsim I2 tid r) top9) (cpn9 (fun r => pind9 (__lsim I2 tid r) top9)).
+  Proof.
+    ss. i.
+    unfold gupaco9 in *.
+    eapply gpaco9_mon_gen. eapply PR. all: i; ss; auto with paco.
+    2:{ inv PR0. econs. 2: apply CLO. inv COM. econs; auto.
+        i. exploit compat9_compat.
+        { eapply compat9_mon. apply PR0. i. eapply _lsim_equivI. 2: apply PR1. clear - EQ. i. rewrite EQ; auto. }
+        { i. eapply _lsim_equivI. 2: apply x29. clear - EQ. i. rewrite EQ; auto. }
+    }
+    { eapply _lsim_equivI. 2: apply PR0. clear - EQ. i. rewrite EQ; auto. }
+  Qed.
+
+End EQUIVI.
 
 Module ModSim.
   Section MODSIM.
